axiomatic `Lexpr_holds`; `sym_stk_eq_stk_frm`

rich_raven_lang/trnsl.v
@@ -52,13 +52,65 @@ Section MainTranslation.
     (* Definition stack_to_stack_frame (stk : stack) : stack_frame := 
     . *)
   
+    Definition sym_stk_eq_stk_frm (stk : stack) (stk_frm : stack_frame) : Prop :=
+      (forall (x : var) (le : LExpr), (stk !! x = Some le) -> (∃ (v : lang.val),  (stk_frm.(locals) !! x = Some v) /\ (LExpr_holds (LBinOp EqOp le (LVal (trnsl_val v)))))) /\
+      
+      (forall (x : var) (v : lang.val), (stk_frm.(locals) !! x = Some v) -> (∃ (le : LExpr), (stk !! x = Some le) /\ (LExpr_holds (LBinOp EqOp le (LVal (trnsl_val v)))))).
+
+    Lemma sym_stk_eq_stk_frm_func (stk : stack) (stk_frm1 : stack_frame) (stk_frm2 : stack_frame) :
+      sym_stk_eq_stk_frm stk stk_frm1 ->
+      sym_stk_eq_stk_frm stk stk_frm2 ->
+      stk_frm1 = stk_frm2.
+    Proof.
+      intros H1 H2.
+      destruct stk_frm1 as [locals1 ].
+      destruct stk_frm2 as [locals2 ].
+      f_equal.
+      apply map_eq .
+
+      destruct H1 as [H1f H1b].
+
+      intros i.
+
+      destruct (locals1 !! i) eqn: Hstkfrm1i.
+      - specialize (H1b i v Hstkfrm1i).
+        destruct H1b as [le [Hstki HLexprH]].
+
+        destruct H2 as [H2f H2b].
+        specialize (H2f i le Hstki).
+        destruct H2f as [v' [Hstkfrm2i HLexprH2]].
+        apply EqOp_refl in HLexprH.
+        pose proof (EqOp_trans _ _ _ HLexprH HLexprH2) as HE.
+        pose proof (EqpOp_LVal _ _ HE) as HE2.
+        apply trnsl_val_inj in HE2.
+        subst v'.
+        simpl in Hstkfrm2i. done.
+      
+      - destruct (stk !! i) eqn: Hstk1i.
+        + specialize (H1f _ _ Hstk1i).
+          destruct H1f as [v [Hstkfrm1]].
+          simpl in Hstkfrm1.
+          rewrite Hstkfrm1 in Hstkfrm1i.
+          inversion Hstkfrm1i.
+
+        + destruct (locals2 !! i) eqn: Hstkfrm2i.
+          * destruct H2 as [H2f H2b].
+            specialize (H2b _ _ Hstkfrm2i).
+            destruct H2b as [le' [Hstk2i _]].
+            rewrite Hstk1i in Hstk2i.
+            inversion Hstk2i.
+          * done.
+    Qed.
+
+
     Definition trnsl_hoare_triple (stk : stack) (stk_frm : stack_frame) (stk_id: stack_id) (p : assertion) (a1 : AtomicAnnotation) (cmd : stmt) (stk' : stack) (stk_frm' : stack_frame) (q : assertion) (a2 : AtomicAnnotation) : iProp rrl_lang.Σ :=
         match (trnsl_stmt cmd stk), (trnsl_assertion p), (trnsl_assertion q) with
         | Error, _, _ | _, None, _ | _, _, None => True
         | None', Some p', Some q' => 
           (p' ∗ trnsl_atomic_annotation (inv_set_to_namespace a1.1) a1) -∗ |={(inv_set_to_namespace a1.1), (inv_set_to_namespace a2.1) }=> (q' ∗ trnsl_atomic_annotation (inv_set_to_namespace a2.1) a2)
         | Some' s, Some p', Some q' => 
-          (* forall (x : Var), trnsl_expressions (stk)-> *)
+          ⌜sym_stk_eq_stk_frm stk stk_frm⌝ -∗
+          ⌜sym_stk_eq_stk_frm stk' stk_frm'⌝ -∗
           {{{ p' ∗ stack_own[ stk_id, stk_frm ] }}}  to_rtstmt stk_id s  {{{ RET lang.LitUnit; q' ∗ stack_own[ stk_id, stk_frm' ] }}}
         end
     .
@@ -72,13 +124,29 @@ Section MainTranslation.
       3: {
         unfold trnsl_hoare_triple.
         destruct (trnsl_stmt (FldWr e1 fld e2) stk) eqn:Ht. 2:{done. }
-        - inversion Ht. 
-        -
+        { inversion Ht. } 
 
-        inversion Ht.
+        inversion Ht. simpl. 
+        destruct (trnsl_lval old_val); destruct (trnsl_lval new_val); simpl; iIntros; try done.
+        - iIntros (Φ). iModIntro.
+        iIntros "[Hstk1 Hstk2] HΦ".
 
-          inversion H3; subst. simpl. destruct H2.
-  
+        iDestruct "Hstk1" as "[%l [%Hlexpr1 Hlfld]]".
+        
+        iApply (wp_heap_wr stk_id stk_frm _ _ _ l _ _ with "[Hstk2 Hlfld]").
+
+
+        2: {
+          iModIntro. iIntros "[HstkO Hlpt]".
+          iApply "HΦ". iFrame.
+          iSplitR. { iPureIntro. done. }
+          pose proof (sym_stk_eq_stk_frm_func _ _ _ H2 H4). subst stk_frm'. iFrame.
+        }
+        
+        1: {
+          iFrame.
+          admit.
+        }
   
     Admitted.
     
